#295, update speedup proof of concept examples:  - init edge is expected to be a Call  - add slightly bigger example

trunk/examples/programs/heapseparator/speedup-poc01-03.bpl
@@ -1,6 +1,7 @@
 //#Safe
 var #memory_int, #valid : [int] int;
 
+
 procedure ULTIMATE.start(); 
 modifies #memory_int, #valid;
 
@@ -14,21 +15,34 @@ procedure main();
 modifies #memory_int, #valid;
 
 implementation main() {
-  var p1, p2, x1, x2 : int;
+  var p1, p2, p3, p4, x1, x2, x3, x4 : int;
 
   assume p1 != p2;
+  assume p1 != p3;
+  assume p1 != p4;
+  assume p2 != p3;
+  assume p2 != p4;
+  assume p3 != p4;
 
   #memory_int[p1] := 0;
   #memory_int[p2] := 0;
+  #memory_int[p3] := 0;
+  #memory_int[p4] := 0;
 
   while (*) {
     if (*) {
       #memory_int[p1] := #memory_int[p1] + 1;
-    } else {
+    } else if (*) {
       #memory_int[p2] := #memory_int[p2] - 1;
+    } else if (*) {
+      #memory_int[p3] := #memory_int[p3] + 1;
+    } else {
+      #memory_int[p4] := #memory_int[p4] - 1;
     }
   }
   assert #memory_int[p1] >= 0;
   assert #memory_int[p2] <= 0;
+  assert #memory_int[p3] >= 0;
+  assert #memory_int[p4] <= 0;
 
 }
